---
slug: math-01
title: Math 01
authors: pitikorn32
tags: [Series, Analysis, sum of infinite series, logarithm, exponential function]
---

# 87-S1-Q4

Show that the sum of the infinite series

$$
\log_{2}\mathrm{e}-\log_{4}\mathrm{e}+\log_{16}\mathrm{e}-\ldots+(-1)^{n}\log_{2^{2^{n}}}\mathrm{e}+\ldots
$$
is
$$
\frac{1}{\ln(2\sqrt{2})}
$$

[ $\log_{a}b=c$ is equivalent to $a^{c}=b$ ]

<!--truncate-->

STEP I 1987 Question 4 (Pure)

## Solution

<details><summary><b>click</b></summary>  

$$
\log_{2}\mathrm{e}-\log_{4}\mathrm{e}+\log_{16}\mathrm{e}-\ldots+(-1)^{n}\log_{2^{2^{n}}}\mathrm{e}+\ldots = \sum_{k=1}^{\infty} (-1)^{k}\log_{2^{2^{k}}}\mathrm{e}
$$

$$
= \sum_{k=1}^{\infty} \frac{(-1)^{k}}{{2^{k}}\ln{2}}
$$

$$
= \frac{1}{\ln{2}}\sum_{k=1}^{\infty} \frac{(-1)^{k}}{2^{k}} = \frac{1}{\ln{2}}\sum_{k=1}^{\infty} {(-\frac{1}{2})}^{k}
$$

$$
= \frac{1}{\ln{2}} \cdot \frac{1}{1 - (-\cfrac{1}{2})} = \frac{1}{\cfrac{3}{2} \cdot \ln{2}}
$$

$$
= \frac{1}{\ln(2\sqrt{2})}
$$

</details>